ListVector completed and refactored

list_vector/ListVectorDef.v
@@ -1,8 +1,8 @@
-Require Import fin_utils.
-Require Import lia_utils.
-Require Import list_utils.
-Require Import Fin.
-Require Import Eqdep_dec Lia.
+Require fin_utils.
+Require lia_utils.
+Require list_utils.
+Require Fin.
+Require Import Lia.
 Require Import Arith_base.
 Import EqNotations.
 Local Open Scope nat_scope.
@@ -14,7 +14,7 @@ Arguments mk_vector {A n}.
 Arguments elts {A n}.
 Arguments elts_spec {A n}.
 
-Definition nil (A : Type) : t A 0 := mk_vector  (Datatypes.nil) eq_refl.
+Definition nil (A : Type) : t A 0 := mk_vector (Datatypes.nil) eq_refl.
 
 Definition cons (A : Type) (h : A) (n : nat) (v : t A n) : t A (S n) :=
   mk_vector (h :: (elts v))%list (f_equal S (elts_spec v)).
@@ -22,32 +22,14 @@ Definition cons (A : Type) (h : A) (n : nat) (v : t A n) : t A (S n) :=
 Local Notation "[ ]" := (nil _) (format "[ ]").
 Local Notation "h :: t" := (cons _ h _ t) (at level 60, right associativity).
 
-Lemma vec_spec_eq: forall {A:Type} {n:nat}, forall (v1 v2: t A n), elts v1 = elts v2 <-> v1 = v2.
-Proof.
-intros A n v1 v2.
-split.
-- intros H.
-  destruct v1 as [el_v1 sp_v1].
-  destruct v2 as [el_v2 sp_v2].
-  cbn in *.
-  destruct H.
-  rewrite (lia_utils.nat_uip sp_v1 sp_v2).
-  reflexivity.
-- intros H.
-  destruct v1 as [el_v1 sp_v1].
-  destruct v2 as [el_v2 sp_v2].
-  apply (f_equal elts) in H.
-  cbn in *.
-  apply H.
-Qed.
-
+Section BASES.
 Definition hd {A:Type} {n:nat} (v:t A (S n)) : A :=
   match elts_spec v with
   | H => 
     match elts v with 
     | l => 
       match l return (length (l) = S n -> A) with
-      | Datatypes.nil => fun H: length Datatypes.nil = S n => match S_not_0 n H  with end 
+      | Datatypes.nil => fun H: length Datatypes.nil = S n => match lia_utils.S_not_0 n H  with end 
       | (h :: t)%list => fun _ => h
       end H
     end
@@ -60,52 +42,33 @@ Qed.
 
 Definition tl {A:Type} {n:nat} (v:t A (S n)) : t A n :=
 {| elts := List.tl (elts v); elts_spec := tl_aux (elts v) (elts_spec v)|}.
+End BASES.
 
-Lemma vec_hd_tl_eq: forall (n:nat) (A:Type) (v:t A (S n)), v = (hd v :: tl v).
-Proof.
-intros n A v.
-destruct v as [l l_sp].
-destruct n, l.
-- cbn in l_sp.
-  destruct (lia_utils.S_not_0 _ l_sp).
-- apply vec_spec_eq.
-  reflexivity.
-- cbn in *.
-  destruct (lia_utils.S_not_0 _ l_sp).
-- apply vec_spec_eq.
-  reflexivity.
-Qed.
 
-Require Import Lia.
+Section SCHEMES.
+
 
 Definition case0 {A} (P:t A 0 -> Type) (H:P (nil A)) v:P v:=
 match v with | {| elts := l; elts_spec := l_sp |} => 
   match l return (forall l_sp, P {| elts := l; elts_spec := l_sp |}) with
   | Datatypes.nil => fun l_sp => 
-    rew <- [fun l_sp => P {| elts := Datatypes.nil; elts_spec := l_sp |}] nat_uip l_sp eq_refl in H
-  | (a :: l)%list => fun l_sp => match S_not_0 _ (eq_sym l_sp) with end
+    rew <- [fun l_sp => P {| elts := Datatypes.nil; elts_spec := l_sp |}] lia_utils.nat_uip l_sp eq_refl in H
+  | (a :: l)%list => fun l_sp => match lia_utils.S_not_0 _ (eq_sym l_sp) with end
   end l_sp
 end.
 
-Lemma nil_spec: forall {A:Type} (v:t A 0), v = nil A.
+Lemma nil_spec {A} (v : t A 0) : v = [].
 Proof.
-intros A v.
-destruct v as [l l_sp].
-destruct l.
-- cbn in *.
-  rewrite (lia_utils.nat_uip l_sp eq_refl).
-  reflexivity.
-- cbn in *.
-  destruct (lia_utils.S_not_0 _ (eq_sym l_sp)).
-Qed.
+apply (fun P E => case0 P E v). reflexivity.
+Defined.
 
 Definition caseS {A} (P : forall {n}, t A (S n) -> Type)
   (H : forall h {n} t, @P n (h :: t)) {n} (v: t A (S n)) : P v :=
 match v with {| elts := l; elts_spec := l_sp |} => 
     match l return (forall l_sp : length l = S n, P {| elts := l; elts_spec := l_sp |}) with
-    | Datatypes.nil => fun l_sp => match S_not_0 n l_sp with end
+    | Datatypes.nil => fun l_sp => match lia_utils.S_not_0 n l_sp with end
     | (a :: l)%list => fun l_sp => 
-          rew [fun e => P {| elts := a :: l; elts_spec := e |}] nat_uip (f_equal S (f_equal pred l_sp)) l_sp in 
+          rew [fun e => P {| elts := a :: l; elts_spec := e |}] lia_utils.nat_uip (f_equal S (f_equal pred l_sp)) l_sp in 
           H a {| elts := l; elts_spec := f_equal pred l_sp |}
     end l_sp
 end.
@@ -115,9 +78,9 @@ Definition caseS' {A} {n : nat} (v : t A (S n)) : forall (P : t A (S n) -> Type)
 (H : forall h t, P (h :: t)), P v :=
 match v with {| elts := l; elts_spec := l_sp |} => fun P H =>
     match l return (forall l_sp : length l = S n, P {| elts := l; elts_spec := l_sp |}) with
-    | Datatypes.nil => fun l_sp => match S_not_0 n l_sp with end
+    | Datatypes.nil => fun l_sp => match lia_utils.S_not_0 n l_sp with end
     | (a :: l)%list => fun l_sp => 
-          rew [fun e => P {| elts := a :: l; elts_spec := e |}] nat_uip (f_equal S (f_equal pred l_sp)) l_sp in 
+          rew [fun e => P {| elts := a :: l; elts_spec := e |}] lia_utils.nat_uip (f_equal S (f_equal pred l_sp)) l_sp in 
           H a {| elts := l; elts_spec := f_equal pred l_sp |}
     end l_sp
 end. 
@@ -126,67 +89,67 @@ Definition caseS'' {A} (P : forall {n}, t A (S n) -> Type)
   {n} (H : forall h t, @P n (h :: t)) (v: t A (S n)) : P v :=
   match v with {| elts := l; elts_spec := l_sp |} =>
       match l return (forall l_sp : length l = S n, P {| elts := l; elts_spec := l_sp |}) with
-      | Datatypes.nil => fun l_sp => match S_not_0 n l_sp with end
-      | (a :: l)%list => fun l_sp => rew [fun e => P {| elts := a :: l; elts_spec := e |}] nat_uip (f_equal S (f_equal pred l_sp)) l_sp in
+      | Datatypes.nil => fun l_sp => match lia_utils.S_not_0 n l_sp with end
+      | (a :: l)%list => fun l_sp => rew [fun e => P {| elts := a :: l; elts_spec := e |}] lia_utils.nat_uip (f_equal S (f_equal pred l_sp)) l_sp in
             H a {| elts := l; elts_spec := f_equal pred l_sp |}
       end l_sp
   end.
 
 Definition rectS {A} (P:forall {n}, t A (S n) -> Type)
-  (bas: forall a: A, P (a :: []))
-  (rect: forall a {n} (v: t A (S n)), P v -> P (a :: v))
-  : forall (n:nat) (v:t A (S n)), P v.
+ (bas: forall a: A, P (a :: []))
+ (rect: forall a {n} (v: t A (S n)), P v -> P (a :: v)) :=
+ fix rectS_fix {n} (v: t A (S n)) : P v := match n return forall (v : t A (S n)), P v with
+ | 0 => caseS'' _ (fun h w => case0 (fun w => P (h :: w)) (bas h) _)
+ | S m => caseS'' _ (fun h w => rect h w (rectS_fix w))
+ end v.
+
+ Lemma vec_spec_eq: forall {A:Type} {n:nat}, forall (v1 v2: t A n), elts v1 = elts v2 <-> v1 = v2.
+ Proof.
+ intros A n v1 v2.
+ split.
+ - intros H.
+   destruct v1 as [el_v1 sp_v1].
+   destruct v2 as [el_v2 sp_v2].
+   cbn in *.
+   destruct H.
+   rewrite (lia_utils.nat_uip sp_v1 sp_v2).
+   reflexivity.
+ - intros H.
+   destruct v1 as [el_v1 sp_v1].
+   destruct v2 as [el_v2 sp_v2].
+   apply (f_equal elts) in H.
+   cbn in *.
+   apply H.
+ Qed.
+
+Lemma eta {A} {n} (v : t A (S n)) : v = hd v :: tl v.
 Proof.
-  refine (fix rectS_fix (n:nat) (v:t A (S n)) : @P n v := _).
-  refine (match n return forall (v : t A (S n)), P n v with
-  | 0 => _
-  | S m => _
-  end v).
-  - refine (caseS'' _ (fun h w => _)).
-    refine (case0 (fun w => P 0 (h :: w)) (bas h) _).
-  - refine (caseS'' _ (fun h w => _)).
-    refine (rect h m w (rectS_fix m w)).
-Defined.
+destruct v as [l l_sp]; destruct n, l; 
+try (apply vec_spec_eq; reflexivity) ; destruct (lia_utils.S_not_0 _ l_sp).
+Qed.
 
 Definition rect2 {A B} 
   (P:forall {n}, t A n -> t B n -> Type)
   (bas : P [] []) 
-  (rect : forall {n:nat} {v1:t A n} {v2:t B n}, P v1 v2 -> forall a b, P (a :: v1) (b :: v2)): forall {n} (v1 : t A n) (v2: t B n), P v1 v2.
-Proof.
-refine (fix rect2_fix {n} (v1 : t A n) : forall v2 : t B n, P n v1 v2 := _).
-refine (fun v2 => _).
-destruct n.
-- rewrite (nil_spec v1). 
-  rewrite (nil_spec v2).
-  apply bas.
-- rewrite (vec_hd_tl_eq _ _ v1).
-  rewrite (vec_hd_tl_eq _ _ v2).
-  specialize (rect2_fix n (tl v1) (tl v2)).
-  apply (rect n (tl v1) (tl v2) rect2_fix (hd v1) (hd v2)).
-Qed.
+  (rect : forall {n:nat} {v1:t A n} {v2:t B n}, P v1 v2 -> forall a b, P (a :: v1) (b :: v2)): forall {n} (v1 : t A n) (v2: t B n), P v1 v2 :=
+  fix rect2_fix {n} (v1 : t A n) : forall v2 : t B n, P v1 v2 :=
+  match n return forall v1:t A n, forall v2, P v1 v2 with
+  | 0 => fun v1 v2 => 
+    rew <- [fun v1 : t A 0 => P v1 v2] nil_spec v1 in
+    rew <- [fun v2 : t B 0 => P [] v2] nil_spec v2 in bas
+  | S n' => fun v1 v2 => 
+    rew <- [fun v1 : t A (S n') => P  v1 v2] eta v1 in
+    rew <- [fun v2 : t B (S n') => P (hd v1 :: tl v1) v2] eta v2 in
+    @rect n' (tl v1) (tl v2) (rect2_fix (tl v1) (tl v2)) (hd v1) (hd v2) 
+  end v1.
 
+End SCHEMES.
 
-Lemma vector_ind : forall (A : Type) (P : forall n : nat, t A n -> Prop),
-  P 0 (nil _) -> (forall (h : A) (n : nat) (v : t A n), P n v -> P (S n) (cons _ h n v)) ->
-  forall (n : nat) (v : t A n), P n v.
-Proof.
-  intros A P H1 H2 n.
-  induction n; cbn.
-  - intros [[|h elts] Helts]; cbn.
-    + destruct Helts.
-      apply H1.
-    + cbn in Helts.
-      lia.
-  - intros [[|h elts] Helts]; cbn.
-    + cbn in Helts.
-      lia.
-    + specialize (H2 h n (mk_vector elts (f_equal pred Helts)) (IHn _)).
-      cbn in H2.
-      replace Helts with (f_equal S (f_equal Nat.pred Helts)).
-      * apply H2.
-      * apply UIP_dec.
-        decide equality.
-Qed.
+Section BASES.
+
+(*as in std*)
+Definition hd_std {A} := @caseS _ (fun n v => A) (fun h n t => h).
+Global Arguments hd {A} {n} v.
 
 Definition last {A:Type} {n:nat} (v:t A (S n)) : A :=
     match elts_spec v with
@@ -194,65 +157,54 @@ Definition last {A:Type} {n:nat} (v:t A (S n)) : A :=
       match elts v with 
       | l => 
         match l return (length (l) = S n -> A) with
-        | Datatypes.nil => fun H: length Datatypes.nil = S n => match S_not_0 n H  with end 
+        | Datatypes.nil => fun H: length Datatypes.nil = S n => match lia_utils.S_not_0 n H  with end 
         | (h :: t)%list => fun _ => List.last t h
         end H
       end
     end. 
 
+(*as in std*)
+Definition last_std {A} := @rectS _ (fun _ _ => A) (fun a => a) (fun _ _ _ H => H).
+Global Arguments last {A} {n} v.
+
 Fixpoint const {A:Type} (a:A) (n:nat): t A n :=
 match n with
-| 0 => nil _
-| S n' => cons _ a n' (const a n')
+| 0 => []
+| S n' =>  a :: (const a n')
 end.
 
-Fixpoint nth_refine {A:Type} {n:nat} (v:t A n) (f:Fin.t n) : A.
-Proof.
-refine (match f in Fin.t n return t A n -> A with | @Fin.F1 n => _ | @Fin.FS n f' => _ end v).
-- refine (fun v => _). 
-  refine (match v with {| elts:=l; elts_spec:=l_sp|} => _ end).
-  refine (match l return length l = S n -> A with | Datatypes.nil => _ | (a::l')%list => _ end l_sp).
-  + refine (fun l_sp => _).
-    refine (match lia_utils.S_not_0 _ l_sp with end).
-  + refine (fun l_sp => _).
-    refine (a).
-- refine (fun v => _).
-  refine (match v with {| elts:=l; elts_spec:=l_sp|} => _ end).
-  refine (match l return length l = S n -> A with | Datatypes.nil => _ | (a::l')%list => _ end l_sp).
-  + refine (fun l_sp => _).
-    refine (match lia_utils.S_not_0 _ l_sp with end).
-  + refine (fun l_sp => _).
-    refine (nth_refine A n ({|elts:=l'; elts_spec:=f_equal pred l_sp |}) f').
-  Show Proof.
-Defined.
+(*as in std*)
+Definition const_std {A} (a:A) := nat_rect _ [] (fun n x => cons _ a n x).
 
-
-Fixpoint nth {A:Type} {n:nat} (v:t A n) (f:Fin.t n) : A := 
-match f in (Fin.t n) return (t A n -> A) with
-  | @F1 n => fun v : t A (S n) => 
-    match v with {| elts := l; elts_spec := l_sp |} => 
-      match l return (length l = S n -> A) with
-      | Datatypes.nil => fun l_sp : length Datatypes.nil = S n => match S_not_0 n l_sp return A with end
-      | (a :: l')%list => fun _ : length (a :: l') = S n => a
-      end l_sp
-    end
-  | @FS n f' => fun v : t A (S n) => 
-    match v with {| elts := l; elts_spec := l_sp |} => 
-      match l return (length l = S n -> A) with
-      | Datatypes.nil => fun l_sp : length Datatypes.nil = S n => match S_not_0 n l_sp return A with end
-      | (a :: l')%list => fun l_sp : length (a :: l') = S n => nth {| elts := l'; elts_spec := f_equal Init.Nat.pred l_sp |} f'
+Fixpoint nth {A:Type} {n:nat} (v:t A n) (f:Fin.t n) : A :=
+match f in Fin.t n return t A n -> A with 
+| @Fin.F1 n => fun v => 
+  match v with {| elts:=l; elts_spec:=l_sp|} => 
+    match l return length l = S n -> A with 
+    | Datatypes.nil => fun l_sp => match lia_utils.S_not_0 _ l_sp with end 
+    | (a::l')%list => fun l_sp =>  a 
     end l_sp
-  end
+  end 
+| @Fin.FS n f' => fun v => 
+  match v with {| elts:=l; elts_spec:=l_sp|} => 
+    match l return length l = S n -> A with 
+    | Datatypes.nil => fun l_sp => match lia_utils.S_not_0 _ l_sp with end 
+    | (a::l')%list => fun l_sp => nth ({|elts:=l'; elts_spec:=f_equal pred l_sp |}) f' 
+    end l_sp
+  end 
 end v.
 
+(*as in std*)
+Definition nth_order {A} {n} (v: t A n) {p} (H: p < n) :=
+(nth v (Fin.of_nat_lt H)).
 
 Definition nth' {A:Type} {n:nat} (v:t A n) (f:Fin.t n) : A :=
 match n return (t A n) -> (Fin.t n) -> A with 
 | 0 => fun (v:t A 0) (f:Fin.t 0) => match f with end
 | S n' => fun (v:t A (S n')) (f:Fin.t (S n')) =>
   match v with 
-  | {| elts := Datatypes.nil ; elts_spec := p |} => match S_not_0 n' p with end
-  | {| elts := (x::xs)%list ; elts_spec := p |} => List.nth (fin_to_nat f) (elts v) x
+  | {| elts := Datatypes.nil ; elts_spec := p |} => match lia_utils.S_not_0 n' p with end
+  | {| elts := (x::xs)%list ; elts_spec := p |} => List.nth (fin_utils.fin_to_nat f) (elts v) x
   end
 end v f.
 
@@ -261,18 +213,23 @@ Proof.
 intros H. cbn in *. assumption.
 Qed.
 
-Fixpoint replace {A:Type} {n:nat} (v:t A n) (f:Fin.t n) (a:A) {struct f} : t A n.
-Proof.
-refine (match f in (Fin.t n) return t A n -> t A n with | @Fin.F1 n' => fun v => _ | @Fin.FS n' f' => fun v => _ end v).
-- refine (match v with {|elts:=l; elts_spec:=l_sp|} => _ end).
-  refine (match l return length l = S n' -> t A (S n') with | Datatypes.nil => fun l_sp => _ | (a'::l')%list => fun l_sp => _ end l_sp).
-  + refine (match lia_utils.S_not_0 _ l_sp with end).
-  + refine ({|elts:= a::l'; elts_spec:=replace_aux a' a l' l_sp|}).
-- refine (match v with {|elts:=l; elts_spec:=l_sp|} => _ end).
-  refine (match l return length l = S n' -> t A (S n') with | Datatypes.nil => fun l_sp => _ | (a'::l')%list => fun l_sp => _ end l_sp).
-  + refine (match lia_utils.S_not_0 _ l_sp with end).
-  + refine (a'::(replace A n' (tl v) f' a)).
-Defined.
+Fixpoint replace {A n} (v : t A n) (p: Fin.t n) (a : A) {struct p}: t A n :=
+match p in (Fin.t n) return t A n -> t A n with 
+| @Fin.F1 n' => fun v => 
+  match v with {|elts:=l; elts_spec:=l_sp|} => 
+    match l return length l = S n' -> t A (S n') with 
+    | Datatypes.nil => fun l_sp => match lia_utils.S_not_0 _ l_sp with end
+    | (a'::l')%list => fun l_sp => {|elts:= a::l'; elts_spec:=replace_aux a' a l' l_sp|}
+    end l_sp 
+  end 
+| @Fin.FS n' f' => fun v => 
+  match v with {|elts:=l; elts_spec:=l_sp|} => 
+    match l return length l = S n' -> t A (S n') with 
+    | Datatypes.nil => fun l_sp => match lia_utils.S_not_0 _ l_sp with end 
+    | (a'::l')%list => fun l_sp => a'::(replace (tl v) f' a)
+    end l_sp  
+  end
+end v.
 
 Lemma replace_aux' {A:Type} {n:nat}: forall (l:list A) (p:length l = n) (i:nat) (a:A), length (list_utils.list_replace l i a) = n.
 Proof.
@@ -283,15 +240,30 @@ Qed.
 
 Definition replace' {A:Type} {n:nat} (v:t A n) (f:Fin.t n) (a:A) : t A n := 
 match v with
-| {| elts := l; elts_spec := p|} => {| elts := (list_replace l (fin_to_nat f) a); elts_spec := (replace_aux' l p (fin_to_nat f) a)|} 
+| {| elts := l; elts_spec := p|} => {| elts := (list_utils.list_replace l (fin_utils.fin_to_nat f) a); elts_spec := (replace_aux' l p (fin_utils.fin_to_nat f) a)|} 
 end.
 
+(*as in std*)
+Definition uncons {A} {n : nat} (v : t A (S n)) : A * t A n := (hd v, tl v).
+
+(*as in std*)
+Definition shiftout {A} := @rectS _ (fun n _ => t A n) (fun a => [])
+  (fun h _ _ H => h :: H).
+Global Arguments shiftout {A} {n} v.
+
+Fixpoint shiftin {A} {n:nat} (a : A) (v:t A n) : t A (S n) :=
+match n return t A n -> t A (S n) with 
+| 0 => fun v => {| elts := (a::Datatypes.nil)%list; elts_spec := eq_refl|}
+| S n' => fun v => (hd v) :: shiftin a (tl v)
+end v.
+
+(*as in std*)
+Definition shiftrepeat {A} := @rectS _ (fun n _ => t A (S (S n)))
+  (fun h =>  h :: h :: []) (fun h _ _ H => h :: H).
+Global Arguments shiftrepeat {A} {n} v.
+
 Lemma take_aux {i n m:nat}: forall (p:i<=n) (H:m = n), i<=m.
-Proof.
-intros.
-rewrite H.
-apply p.
-Qed.
+Proof. intros. rewrite H. apply p. Qed.
 
 Definition take {A:Type} {n:nat} : forall i : nat, (i <= n) -> t A n -> t A i :=
 fun (i:nat) (p:i <= n) (v: t A n) =>
@@ -300,6 +272,19 @@ match v with
   {|elts := List.firstn i l; elts_spec := (List.firstn_length_le l (take_aux p s))|}
 end.
 
+(*as in std*)
+Lemma trunc : forall {A} {n} (p:nat), n > p -> t A n
+  -> t A (n - p).
+Proof.
+  intros A n p; induction p as [| p f]; intros H v.
+  - rewrite Nat.sub_0_r.
+    exact v.
+  - apply shiftout.
+    rewrite <- Nat.sub_succ_l.
+    + exact (f (Nat.lt_le_incl _ _ H) v).
+    + exact (Nat.lt_le_incl _ _ H).
+Defined.
+
 Lemma append_aux{x n m n' m': nat}: forall(pn:n = n') (pm: m = m') (H: x = n + m), x = n' + m'.  
 Proof. lia. Qed.
 
@@ -307,69 +292,135 @@ Definition append {A:Type} {n:nat} {p:nat} (v:t A n) (w:t A p) : t A (n + p) :=
 match v with {| elts := elts_v; elts_spec := elts_spec_v |} => match w with {| elts := elts_w ; elts_spec:=elts_spec_w|} => 
   {|elts := elts_v ++ elts_w; elts_spec := append_aux elts_spec_v elts_spec_w (List.app_length elts_v elts_w)|} end end.
 
+(*as in std*)
+Fixpoint splitat {A} (l : nat) {r : nat} :
+  t A (l + r) -> t A l * t A r :=
+  match l with
+  | 0 => fun v => ([], v)
+  | S l' => fun v =>
+    let (v1, v2) := splitat l' (tl v) in
+    (hd v::v1, v2)
+  end.
+
+Fixpoint rev_append_tail {A n p} (v : t A n) (w: t A p)
+  : t A (Nat.tail_add n p) :=
+  match n return t A n -> t A (Nat.tail_add n p) with 
+  | 0 => fun v => w 
+  | S n' => fun v => rev_append_tail (tl v) ((hd v) :: w)
+  end v.
+
+(*as in std*)
+Definition rev_append {A n p} (v: t A n) (w: t A p)
+  :t A (n + p) :=
+  rew (Nat.tail_add_spec n p) in (rev_append_tail v w).
+
 Definition rev {A:Type} {n:nat} (v:t A n) : t A n := 
 match v with {|elts:=l;elts_spec:=p|} => 
 {|elts:= List.rev l ; elts_spec:= eq_trans (List.rev_length l) p |}
 end.
 
-Definition map {A:Type} {B:Type} (f:A->B) : forall n: nat, t A n -> t B n :=
-fun (n:nat) (v:t A n) => 
+(*as in std*)
+Definition rev_std {A n} (v : t A n) : t A n :=
+ rew <- (plus_n_O _) in (rev_append v []).
+
+End BASES.
+Local Notation "v [@ p ]" := (nth v p) (at level 1).
+
+
+Section ITERATORS.
+
+Definition map {A} {B} (f : A -> B) : forall {n} (v:t A n), t B n := fun (n:nat) (v:t A n) => 
 match v with {|elts:=l;elts_spec:=p|} => 
 {|elts:=List.map f l; elts_spec:= eq_trans (List.map_length f l) p|}
 end.
 
-Definition fold_right {A:Type} {B:Type} (f:A->B->B) : forall n:nat, t A n -> B -> B :=
-fun (n:nat) (v:t A n) (b:B) =>
-match v with {|elts:=l;elts_spec:=p|} => 
-List.fold_right f b l
-end.
+(*as in std*)
+Definition map2 {A B C} (g:A -> B -> C) :
+  forall (n : nat), t A n -> t B n -> t C n :=
+@rect2 _ _ (fun n _ _ => t C n) (nil C) (fun _ _ _ H a b => (g a b) :: H).
+Global Arguments map2 {A B C} g {n} v1 v2.
+
+Definition fold_left {A B:Type} (f:B->A->B): forall (b:B) {n} (v:t A n), B :=
+  fix fold_left_fix (b:B) {n} (v : t A n) : B :=
+    match n return t A n -> B with
+    | 0 => fun v => b
+    | S n' => fun v => (fold_left_fix (f b (hd v)) (tl v))
+    end v.
+
+Definition fold_right {A B : Type} (f : A->B->B) :=
+fun {n:nat} (v:t A n) (b:B) => match v with {|elts:=l;elts_spec:=p|} => List.fold_right f b l end.
+
+(*as in std*)
+Definition fold_right2 {A B C} (g:A -> B -> C -> C) (c: C) :=
+@rect2 _ _ (fun _ _ _ => C) c (fun _ _ _ H a b => g a b H).
+
+Definition fold_left2 {A B C: Type} (f : A -> B -> C -> A) :=
+fix fold_left2_fix (a : A) {n} (v : t B n) : t C n -> A := 
+match n return t B n -> t C n -> A with
+| 0 => fun v w => case0 (fun _ => A) a w
+| S n' => fun v w => caseS' w (fun _ => A) (fun wh wt => fold_left2_fix (f a (hd v) (hd w)) (tl v) (tl w))
+end v. 
+
+End ITERATORS.
+
+(*as in std*)
+Section SCANNING.
+Inductive Forall {A} (P: A -> Prop): forall {n} (v: t A n), Prop :=
+ |Forall_nil: Forall P []
+ |Forall_cons {n} x (v: t A n): P x -> Forall P v -> Forall P (x::v).
+#[local]
+Hint Constructors Forall : core.
+
+Inductive Exists {A} (P:A->Prop): forall {n}, t A n -> Prop :=
+ |Exists_cons_hd {m} x (v: t A m): P x -> Exists P (x::v)
+ |Exists_cons_tl {m} x (v: t A m): Exists P v -> Exists P (x::v).
+#[local]
+Hint Constructors Exists : core.
+
+Inductive In {A} (a:A): forall {n}, t A n -> Prop :=
+ |In_cons_hd {m} (v: t A m): In a (a::v)
+ |In_cons_tl {m} x (v: t A m): In a v -> In a (x::v).
+#[local]
+Hint Constructors In : core.
+
+Inductive Forall2 {A B} (P:A->B->Prop): forall {n}, t A n -> t B n -> Prop :=
+ |Forall2_nil: Forall2 P [] []
+ |Forall2_cons {m} x1 x2 (v1:t A m) v2: P x1 x2 -> Forall2 P v1 v2 ->
+    Forall2 P (x1::v1) (x2::v2).
+#[local]
+Hint Constructors Forall2 : core.
+
+Inductive Exists2 {A B} (P:A->B->Prop): forall {n}, t A n -> t B n -> Prop :=
+ |Exists2_cons_hd {m} x1 x2 (v1: t A m) (v2: t B m): P x1 x2 -> Exists2 P (x1::v1) (x2::v2)
+ |Exists2_cons_tl {m} x1 x2 (v1:t A m) v2: Exists2 P v1 v2 -> Exists2 P (x1::v1) (x2::v2).
+#[local]
+Hint Constructors Exists2 : core.
+
+End SCANNING.
+
+Section VECTORLIST.
 
 Definition of_list {A:Type} : forall l : list A, t A (length l) := 
 fun (l:list A) =>
 {| elts := l; elts_spec := eq_refl |}.
+
+(*as in std*)
+Fixpoint of_list_std {A} (l : list A) : t A (length l) :=
+match l as l' return t A (length l') with
+  |Datatypes.nil => []
+  |(h :: tail)%list => (h :: (of_list_std tail))
+end.
 
 Definition to_list {A:Type} {n:nat} (v:t A n) : list A :=
 match v with {|elts:=l;elts_spec:=p|} => 
 l
 end.
 
+Definition to_list_std {A}{n} (v : t A n) : list A :=
+Eval cbv delta beta in fold_right (fun h H => Datatypes.cons h H) v Datatypes.nil.
 
+End VECTORLIST.
 
-
-
-
-
-
-
-
-
-
-
-
-
-
-(*others*)
-Definition hd' {A:Type} {n:nat} (v:t A n) : option A :=
-match (elts v) with
-| Datatypes.nil => None
-| (x::l)%list => Some x
-end.
-
-
-Definition tl' {A:Type} {n:nat} (v:t A n) : t A (pred n):=
-match n return (t A n -> t A (pred n)) with
-| 0 => fun (v':t A 0) => nil _
-| S m' as m => fun (v':t A m) =>
-    match v' with
-    | {|elts := l; elts_spec := H |} => mk_vector (List.tl l) (tl_aux l H)
-    end
-end v.
-
-Definition last' {A:Type} {n:nat} (v:t A n ) : option A := 
-match elts v with
-| Datatypes.nil => None
-| (h::t)%list => Some(List.last t h)
-end.
 
 Module ListVectorNotations.
 Declare Scope list_vector_scope.
